deps/poulet4/lib/Semantics.v
@@ -1723,7 +1723,7 @@ Definition instantiate'' (ce : cenv) (e : ienv) (typ : @P4Type tags_t)
   if is_decl_extern_obj decl then
     let m := map_fst (map_fst (PathMap.set p (mk_inst_ref class_name p))) m in
     let type_params := get_type_params typ in
-    let (ee, s) := alloc_extern (snd m) s class_name type_params p (map ienv_val_to_sumtype args) in
+    let (ee, s) := construct_extern (snd m) s class_name type_params p (map ienv_val_to_sumtype args) in
     (inl (mk_inst_ref class_name p), m, s)
   else
     let e := IdentMap.sets params args e in
